tests/NormSimp.lean
@@ -1,0 +1,19 @@
+/-
+Copyright (c) 2022 Jannis Limperg. All rights reserved.
+Released under Apache 2.0 license as described in the file LICENSE.
+Authors: Jannis Limperg
+-/
+
+import Aesop
+
+set_option aesop.check.all true
+
+-- A basic test for local simp rules.
+example {α : Prop} (h : α) : α := by
+  fail_if_success aesop (rule_sets [-builtin,-default])
+  aesop (rule_sets [-builtin,-default]) (add h norm simp)
+
+-- This test checks that we don't 'self-simplify' hypotheses: `h` should not
+-- be used to simplify itself.
+example (h : (α ∧ β) ∨ γ) : α ∨ γ := by
+  aesop (add h norm simp)
